Remove index set from hml datatype definition

HML/HML.thy
@@ -1,45 +1,43 @@
 theory HML
-  imports Main "../LTS"
+  imports Main "HOL-Library.Countable_Set_Type" "../LTS"
 begin
 
 datatype 
-  ('act, 'i) hml =
-    TT |
-    Obs 'act "('act, 'i) hml" |
-    Silent "('act, 'i) hml" |
-    Internal "('act, 'i) hml" |
-    Conj "'i set" "'i \<Rightarrow> ('act, 'i) hml_conjunct"
+  'act hml =
+    Obs 'act "'act hml" |
+    Silent "'act hml" |
+    Internal "'act hml" |
+    Conj "'act hml_conjunct cset"
 and
-  ('act, 'i) hml_conjunct =
-    Pos "('act, 'i) hml" |
-    Neg "('act, 'i) hml"
+  'act hml_conjunct =
+    Pos "'act hml" |
+    Neg "'act hml"
 
-
+abbreviation "TT \<equiv> Conj cempty"
 
 context LTS_Tau
 begin
 
 function
-      hml_models     :: "('a, 's) hml     \<Rightarrow> 's \<Rightarrow> bool" ("_ \<Turnstile> _" 60) 
-  and hml_neg_models :: "('a, 's) hml_conjunct \<Rightarrow> 's \<Rightarrow> bool"
+      hml_models     :: "'a hml          \<Rightarrow> 's \<Rightarrow> bool" ("_ \<Turnstile> _" 60) 
+  and hml_neg_models :: "'a hml_conjunct \<Rightarrow> 's \<Rightarrow> bool"
 where
-  "(TT           \<Turnstile> _) = True" |
   "((Obs a \<phi>)    \<Turnstile> p) = (\<exists>p'. p \<mapsto> a p' \<and> (\<phi> \<Turnstile> p'))" |
   "((Silent \<phi>)   \<Turnstile> p) = (\<exists>p'. p \<Zsurj> p' \<and> (\<phi> \<Turnstile> p'))" |
   "((Internal \<phi>) \<Turnstile> p) = ((\<exists>p'. p \<mapsto> \<tau> p' \<and> (\<phi> \<Turnstile> p')) \<or> (\<phi> \<Turnstile> p))" |
-  "((Conj I \<psi>s)  \<Turnstile> p) = (\<forall>i \<in> I. hml_neg_models (\<psi>s i) p)" |
+  "((Conj \<psi>s)    \<Turnstile> p) = (\<forall>\<psi>. cin \<psi> \<psi>s \<longrightarrow> (hml_neg_models \<psi> p))" |
 
   "(hml_neg_models (Pos \<phi>) p) = (\<phi> \<Turnstile> p)" |
   "(hml_neg_models (Neg \<phi>) p) = (\<not>(\<phi> \<Turnstile> p))"
   by (metis hml.exhaust hml_conjunct.exhaust sumE surj_pair, auto)
-            
-inductive_set hml_models_wf_arg_space :: "(('a, 's) hml \<times> 's, ('a, 's) hml_conjunct \<times> 's) sum rel" where
-                          "(Inl (\<phi>, x), Inl (Obs    a \<phi>, p)) \<in> hml_models_wf_arg_space" |
-                          "(Inl (\<phi>, x), Inl (Silent   \<phi>, p)) \<in> hml_models_wf_arg_space" |
-                          "(Inl (\<phi>, x), Inl (Internal \<phi>, p)) \<in> hml_models_wf_arg_space" |
-  "i \<in> I \<Longrightarrow> \<psi> = \<psi>s i \<Longrightarrow> (Inr (\<psi>, p), Inl (Conj  I \<psi>s, p)) \<in> hml_models_wf_arg_space" |
-                          "(Inl (\<phi>, p), Inr (Pos      \<phi>, p)) \<in> hml_models_wf_arg_space" |
-                          "(Inl (\<phi>, p), Inr (Neg      \<phi>, p)) \<in> hml_models_wf_arg_space"
+
+inductive_set hml_models_wf_arg_space :: "('a hml \<times> 's, 'a hml_conjunct \<times> 's) sum rel" where
+                "(Inl (\<phi>, x), Inl (Obs    a \<phi>, p)) \<in> hml_models_wf_arg_space" |
+                "(Inl (\<phi>, x), Inl (Silent   \<phi>, p)) \<in> hml_models_wf_arg_space" |
+                "(Inl (\<phi>, x), Inl (Internal \<phi>, p)) \<in> hml_models_wf_arg_space" |
+  "cin \<psi> \<psi>s \<Longrightarrow> (Inr (\<psi>, p), Inl (Conj    \<psi>s, p)) \<in> hml_models_wf_arg_space" |
+                "(Inl (\<phi>, p), Inr (Pos      \<phi>, p)) \<in> hml_models_wf_arg_space" |
+                "(Inl (\<phi>, p), Inr (Neg      \<phi>, p)) \<in> hml_models_wf_arg_space"
 
 lemma wf_hml_models_wf_arg_space: "wf hml_models_wf_arg_space"
   unfolding wf_def
@@ -49,43 +47,39 @@ proof safe
 
   then show "P \<phi>sOr\<psi>s"
   proof (induct \<phi>sOr\<psi>s)
-    fix \<phi>s :: "('a, 's) hml \<times> 's"
+    fix \<phi>s :: "'a hml \<times> 's"
     obtain \<phi> and sl where "\<phi>s = (\<phi>, sl)" by fastforce
 
-    fix \<psi>s :: "('a, 's) hml_conjunct \<times> 's"
+    fix \<psi>s :: "'a hml_conjunct \<times> 's"
     obtain \<psi> and sr where "\<psi>s = (\<psi>, sr)" by fastforce
 
     show "P (Inl \<phi>s)" and "P (Inr \<psi>s)"
       unfolding \<open>\<phi>s = (\<phi>, sl)\<close> and \<open>\<psi>s = (\<psi>, sr)\<close>
       using \<open>\<forall>x. (\<forall>y. (y, x) \<in> hml_models_wf_arg_space \<longrightarrow> P y) \<longrightarrow> P x\<close>
     proof (induct \<phi> and \<psi> arbitrary: sl and sr)
-      case TT
-      then show ?case
-        by (smt (verit) hml.distinct(1) hml.distinct(3) hml.distinct(5) hml.distinct(7) Inl_inject Pair_inject hml_models_wf_arg_space.simps sum.distinct(1))
-    next
       case (Obs x1 x2)
       then show ?case
-        by (smt (verit) hml.distinct(11) hml.distinct(13) hml.distinct(9) hml.inject(1) Inl_inject Pair_inject hml_models_wf_arg_space.simps sum.distinct(1))
+        by (smt (verit) Inl_inject Inr_not_Inl Pair_inject hml.distinct(1) hml.distinct(3) hml.distinct(5) hml.inject(1) hml_models_wf_arg_space.cases)
     next
       case (Silent x)
       then show ?case
-        by (smt (verit) hml.distinct(15) hml.distinct(17) hml.distinct(9) hml.inject(2) Inl_inject Pair_inject hml_models_wf_arg_space.simps sum.distinct(1))
+        by (smt (verit) Inl_inject Inr_not_Inl Pair_inject hml.distinct(1) hml.distinct(7) hml.distinct(9) hml.inject(2) hml_models_wf_arg_space.cases)
     next
       case (Internal x)
       then show ?case
-        by (smt (verit) hml.distinct(11) hml.distinct(15) hml.distinct(19) hml.inject(3) Inl_inject Pair_inject hml_models_wf_arg_space.simps sum.distinct(1))
+        by (smt (verit) Inl_inject Inr_not_Inl Pair_inject hml.distinct(11) hml.distinct(3) hml.distinct(7) hml.inject(3) hml_models_wf_arg_space.cases)
     next
-      case (Conj x1 x2)
+      case (Conj x)
       then show ?case
-        by (smt (verit) hml.distinct(13) hml.distinct(17) hml.distinct(19) hml.inject(4) Inl_inject Pair_inject hml_models_wf_arg_space.simps range_eqI sum.distinct(1))
+        by (smt (verit) Inl_inject Inr_not_Inl Pair_inject hml.distinct(11) hml.distinct(5) hml.distinct(9) hml.inject(4) hml_models_wf_arg_space.cases cin.rep_eq)
     next
       case (Pos x)
       then show ?case
-        by (smt (verit) hml_conjunct.distinct(1) hml_conjunct.inject(1) Inr_inject Pair_inject hml_models_wf_arg_space.simps sum.distinct(1))
+        by (smt (verit) Inr_inject Inr_not_Inl Pair_inject hml_conjunct.distinct(1) hml_conjunct.inject(1) hml_models_wf_arg_space.cases)
     next
       case (Neg x)
       then show ?case
-        by (smt (verit) hml_conjunct.distinct(2) hml_conjunct.inject(2) Inr_inject Pair_inject hml_models_wf_arg_space.simps sum.distinct(1))
+        by (smt (verit) Inr_inject Inr_not_Inl Pair_inject hml_conjunct.distinct(1) hml_conjunct.inject(2) hml_models_wf_arg_space.cases)
     qed
   qed
 qed
@@ -93,6 +87,11 @@ qed
 termination
   using wf_hml_models_wf_arg_space
   by (standard) (simp add: hml_models_wf_arg_space.intros)+
+
+lemma TT_admits_all_states:
+  fixes p::'s
+  shows "TT \<Turnstile> p"
+  by simp
 
 end
 
